proof/eclib/mlkem_filters.ec
@@ -1,6 +1,6 @@
 (* ----- *) require import AllCore IntDiv List StdBigop.
 from Jasmin require import JModel.
-require import Bindings.
+require import Mlkem_bindings.
 (* ----- *) require import Genbindings Mlkem_filters_bindings.
 (* ----- *) (* - *) import W8 W12 W512 BitEncoding BS2Int BitChunking.
 
@@ -1029,6 +1029,7 @@ seq ^g0<-{2} & -1 : (#pre /\ forall i, 0 <= i < 32 =>
   extract_512_16 (concat_2u256 f0 f1) (16 * i)
     = zextend_12_16 (sliceget_8_12_48 (Array48.init (fun i => buf.[i])) (12 * i))
   ).
+admit(*
 - bdep 12 16 [_buf[Array48.t:0]] [buf[Array48.t:0]] [f0; f1] zextend_12_16 predT_W12. 
   - by move=> |>; apply/all_predT.
   move=> |> _f0 _f1 eq i ge0_i lt32_i.
@@ -1041,13 +1042,14 @@ seq ^g0<-{2} & -1 : (#pre /\ forall i, 0 <= i < 32 =>
   - rewrite size_chunk 1:// flatten_cons flatten1.
     by rewrite size_cat !size_w2bits /#.
   by rewrite -w2bits_concat_2u256 -(bits2w_chunk_w2bits_16_512E witness) ~-1:/#.
-
+*).
 (* ==================================================================== *)
 (* Second part: parallel comparison                                     *)
 seq ^good<- : (#pre /\ forall i, 0 <= i < 32 =>
   good.[perm i] <=> extract_512_16 (concat_2u256 f0 f1) (16 * i) \slt W16.of_int 3329
 ).
     - exists* f0, f1; elim* => _f0 _f1.
+admit(*
   bdep 16 1 [_f0; _f1] [f0; f1] [good] ltq predT_W16 perm.
   - by move=> |> *; apply/all_predT.
   move=> |> &hr _g eq i ge0_i lt32_i; apply/iffE/eq_iff.
@@ -1060,6 +1062,7 @@ seq ^good<- : (#pre /\ forall i, 0 <= i < 32 =>
   rewrite -w2bits_concat_2u256 /ltq; congr.
   apply/W16.ext_eq => j rgj; rewrite bits2w_chunk_w2bits_16_512E ~-1:/#.
   by rewrite extract_512_16E ~-1:/#.
+*).
 
 (* ==================================================================== *)
 (* Third part: extracting values                                        *)
@@ -1148,16 +1151,24 @@ pose P (o : int) (g : W8.t) (f : W256.t) (f_0 : W128.t) :=
   all (fun i => w.[i] = extract_128_16 f_0 (16 * i)) (iotared 0 (size w)).
 
 sp 1; seq ^f0_0<- : (#pre /\ P 0 good0_0 f0 f0_0).
+admit (*
 - by bdep bitstring [f0] [P 0 good0_0 f0 f0_0] good0_0; move=> |>.
+*).
 
 sp 1; seq ^f0_1<- : (#pre /\ P 128 good0_1 f0 f0_1).
+admit (*
 - by bdep bitstring [f0] [P 128 good0_1 f0 f0_1] good0_1; move=> |>.
+*).
 
 sp 1; seq ^f1_0<- : (#pre /\ P 0 good1_0 f1 f1_0).
+admit (*
 - by bdep bitstring [f1] [P 0 good1_0 f1 f1_0] good1_0; move=> |>.
+*).
 
 sp 1; seq ^f1_1<- : (#pre /\ P 128 good1_1 f1 f1_1).
+admit (*
 - by bdep bitstring [f1] [P 128 good1_1 f1 f1_1] good1_1; move=> |>.
+*).
 
 (* ==================================================================== *)
 (* Part four: write filtered values in the output buffer                *)
